%Magnetohydrodynamics:
\begin{eqnarray*}
    \partial_t \rho+\nabla\Cdot(\vv\rho)&=& 0
\\
    \partial_t(\rho\vv)+\nabla\Cdot(\vv\rho\vv-\BB\BB)+\nabla p_{tot}&=& 
       -(\nabla\Cdot\BB)\BB
\\
    \partial_t e+\nabla\Cdot(\vv e-\BB\BB\Cdot\vv+\vv p_{tot})&=& 
       -(\nabla\Cdot\BB)\BB\Cdot\vv+\nabla\Cdot(\BB\times\eta\JJ)
\\
   \partial_t \BB+\nabla\Cdot(\vv\BB-\BB\vv)&=&
       -(\nabla\Cdot\BB)\vv-\nabla\times(\eta\JJ) 
\end{eqnarray*}
\null
\begin{displaymath}
p=(\gamma-1)(e-\rho\vv^2/2-\BB^2/2)~~~~~p_{tot}=p+\BB^2/2~~~~~\JJ=\nabla\times\BB
\end{displaymath}
